Update demos

apps/tc/demo/2023_31_07-byalistock/demo3_sort.v
@@ -1,22 +1,22 @@
 From elpi.apps.tc.tests.premisesSort Require Import sortCode.
 Elpi Debug "simple-compiler".
 
-Class A (S : Type) (T : Type).
-Class B (S : Type) (T : Type).
-Class C (S : Type).
+Class C1 (S : Type) (T : Type).
+Class C2 (S : Type).
+Class C3 (S : Type).
 
-Global Hint Mode A + - : typeclass_instances.
-Global Hint Mode B + - : typeclass_instances.
+Global Hint Mode C1 + - : typeclass_instances.
+Global Hint Mode C2 + : typeclass_instances.
+Global Hint Mode C3 + : typeclass_instances.
 Elpi AddAllClasses. 
 
-Global Instance A1 : A nat nat. Admitted.
-Global Instance B1 : B nat nat. Admitted.
-
-Global Instance C1 {S T : Type} `{B S T, A T S} : C T. Admitted.
+Global Instance Inst1 : C1 nat nat. Qed.
+Global Instance Inst2 T1 `(C1 T1 T1) : C2 T1. Qed.
+Global Instance Inst3 T1 T2 `(C2 T2, C1 T1 T2) : C3 T1. Qed.
 
 Elpi AddAllInstances.
 Elpi Override TC TC_solver All.
-Goal C nat.
+Goal C3 nat.
   apply _.
 Qed.
 
@@ -24,5 +24,5 @@ Qed.
 (* Global Instance C2 {S T : Type} `{A T S, B S T} : C bool. Admitted. *)
 (* Elpi AddInstances C2. *)
 
-(* Global Instance C3 {S T : Type} `{B T S} : C S. Admitted. *)
+Global Instance C3 {S T : Type} `{B T S} : C S. Admitted.
 (* Elpi AddInstances C3. *)
